\documentclass{article}
\usepackage{lplfitch}
\begin{document}
\fitchprf{\pline[1.]{(A \lor B) \land (\lnot B \lor C)}\\
\pline[2.]{\lnot C}}
{
\subproof{\pline[3.]{\lnot A}}
{
\pline[4.]{A \lor B}[\lande{1}]\\
\pline[5.]{\lnot B \lor C}[\lande{1}]\\
\subproof{\pline[6.]{A}}
{
\pline[7.]{\lfalse}[\lfalsei{6}{3}]\\
\pline[8.]{B}[\lfalsee{7}]
}
\subproof{\pline[9.]{B}}
{
\pline[10.]{B}[\reit{9}]
}
\pline[11.]{B}[\lore{6--8}{9--10}{4}]\\
\subproof{\pline[12.]{\lnot B}}
{
\pline[13.]{\lfalse}[\lfalsei{12}{8}]\\
\pline[14.]{C}[\lfalsee{13}]
}
\subproof{\pline[15.]{C}}
{
\pline[16.]{\lfalse}[\lfalsei{15}{2}]\\
\pline[17.]{\lnot B}[\lfalsee{16}]
}
\pline[18.]{\lfalse}[\lore{12--14}{15--17}{5}]
}
\pline[19.]{\lnot \lnot A}[\lnoti{3--18}]\\
\pline[20.]{A}[\lnote{19}]}
\end{document}